

**QUADRATIC FORMULA**

If  $ax^2 + bx + c = 0$ , then  $x = \frac{-b \pm \sqrt{b^2 - 4ac}}{2a}$

**Remark:** Notice that the equation must be set equal to zero first!

**THE DISCRIMINANT**

**Definition:** For the quadratic equation  $ax^2 + bx + c = 0$ , the discriminant is  $b^2 - 4ac$ .

---

If  $b^2 - 4ac > 0$  and is a perfect square, then  $ax^2 + bx + c = 0$  has two real and rational solutions.  
*(to solve the equation we can use quadratic formula or algebraically)*

If  $b^2 - 4ac > 0$  but is not a perfect square, then  $ax^2 + bx + c = 0$  has two irrational solutions.  
*(to solve the equation we need to use quadratic formula)*

---

If  $b^2 - 4ac = 0$ , then  $ax^2 + bx + c = 0$  has one real and rational solution.

*(to solve the equation we can use quadratic formula or algebraically)*

---

If  $b^2 - 4ac < 0$ , then  $ax^2 + bx + c = 0$  has no real solution but it has two complex solutions  
 (involving the imaginary number ).

*(to solve the equation we need to use quadratic formula)*

---

**Directions: Solve each equation by factoring.**

1.

$$x^2 + 9x = 0$$

**You try!**

2  $4x^2 - 8x = 0$

3  $9x^2 - 25 = 0$

**You try!**

4

$$81x^2 - 1 = 0$$

5

$$x^2 - 10x + 21 = 0$$

*Method – 2: Algebraically*

$$x^2 - 10x + 21 = 0$$

6

$$x^2 + 2x - 80 = 0$$

*Method – 2: Algebraically*

$$x^2 + 2x - 80 = 0$$

**You try!**

7  $x^2 + 9x + 20 = 0$

## You try!

*Method – 2: Algebraically*

$$x^2 + 9x + 20 = 0$$

## You try!

8  $x^2 + 6x - 72 = 0$

**You try!**

$$x^2 + 6x - 72 = 0$$

9

$$2x^2 + 21x + 10 = 0$$

9

$$2x^2 + 21x + 10 = 0$$

10

$$3x^2 + 10x - 8 = 0$$



$$3x^2 + 10x - 8 = 0$$

11

$$4x^2 - 12x + 9 = 0$$

**You try!**

$$4x^2 - 12x + 9 = 0$$

**You try!**

12

$$4x^2 + 5x - 3 = 0$$

**You try!**

13

$$3x^2 + 4x + 8 = 0$$

**You try!*****Example:***

A parallelogram has a base that is 4 units shorter than its height,  $h$ . If the height is increased by 5 units and the base is increased by 3 units, write the expression for the new area,  $A$ , of the parallelogram in square units.

A.  $A = (h - 1)(h + 5)$

B.  $A = (h + 3)(h + 4)$

C.  $A = (h - 1)(h + 4)$

D.  $A = (h + 3)(h + 5)$

**Example:**

Emily tossed a soccer ball straight up into the air. The height of the soccer ball at different times after it was thrown is shown in the table below.

Time(seconds)	Height(feet)
1	25
2	36
3	32
4	10

The height  $h(t)$  of the ball as a function of time can be described by:

$$h(t) = -10t^2 + 40t - 5$$

At which of the following times was the ball located exactly at a height of 30 feet?

A. 3.2 seconds

B. 2.7 seconds

C. 2.1 second

D. 1.6 seconds

**Difference of Squares**

**Formula:**  $a^2 - b^2 = (a - b)(a + b)$

**Difference and Sum of Cubes****Difference of Cubes:**

$$a^3 - b^3 = (a - b)(a^2 + ab + b^2)$$

**Sum of cubes:**

$$a^3 + b^3 = (a + b)(a^2 - ab + b^2)$$

***Examples: Difference of squares***

1.  $m^2 - n^2$

5.  $4x^2 - 9y^2$

2.  $x^2 - 49$

6.  $16m^2 - 49n^2$

3.  $36 - y^2$

4.  $64x^2 - y^2$ 

---

***Examples: Sum and Difference of cubes***

1.  $x^3 - 8$

5.  $27x^3 - 125$

2.  $x^3 + 64$

6.  $64m^3 + 216$

3.  $27 - 8y^3$

4.  $64x^3 - 27$